equiv pref pavx2_cf

proof/crypto_stream/chacha20/ref/ChaCha20_pref.ec
@@ -89,43 +89,10 @@ module M = {
     return (output, plain, len);
   }
 
-(*  
-  proc store32 (output:W64.t, plain:W64.t, len:W32.t, k:W32.t Array16.t) : W64.t * W64.t * W32.t = {
-    var i:int;
-    var k1: W32.t Array16.t;
-    i <- 0;
-    while (i < 16) {
-      k1.[i] <- k.[i] `^` loadW32 Glob.mem (plain + W64.of_int (4 * i));
-      i <- i + 1;
-    }
-    i <- 0;
-    while (i < 16) {
-      Glob.mem <- storeW32 Glob.mem (output + W64.of_int (4 * i)) k1.[i];
-      i <- i + 1;
-    }
-    (output, plain, len) <@ update_ptr (output, plain, len, 64);
-    return (output, plain, len);
-  }
-*)
-(*  proc store32 (output:W64.t, plain:W64.t, len:W32.t, k:W32.t Array16.t) : W64.t * W64.t * W32.t = {
-    
-    var i:int;
-    
-    i <- 0;
-    
-    while ((i < 16)) {
-      Glob.mem <-
-      storeW32 Glob.mem (output + (W64.of_int (4 * i))) (k.[i] `^` (loadW32 Glob.mem (plain + (W64.of_int (4 * i)))));
-      i <- (i + 1);
-    }
-    (output, plain, len) <@ update_ptr (output, plain, len, 64);
-    return (output, plain, len);
-  }
-*)
-
   proc store (output plain: address, len: int, k:W32.t Array16.t) : address * address * int = {
     var i:int;
     var k8_0, k8: WArray64.t;
+    k8 <- witness;
     k8_0 <- WArray64.init32 (fun i => k.[i]);
     i <- 0;  
     while (i < min 64 len) {
